Renaming in progress, fixup for bug #40

Hybrid/OkLib.v
@@ -15,10 +15,10 @@ Section Definitions.
 
 Variables A B : Type.
 
-Inductive ok_LF: list (var * A) -> list var -> Prop :=
-| ok_nil: forall U, ok_LF nil U
+Inductive ok_Hyb: list (var * A) -> list var -> Prop :=
+| ok_nil: forall U, ok_Hyb nil U
 | ok_step: forall w C G U,
-  ~ Mem w U -> ok_LF G (w::U) -> ok_LF ((w, C)::G) U
+  ~ Mem w U -> ok_Hyb G (w::U) -> ok_Hyb ((w, C)::G) U
 .
 
 (* Copied from standard list, but this one uses List from LibList *)
@@ -66,9 +66,9 @@ Tactic Notation "rew_flat_map" "in" hyp(H) :=
 Tactic Notation "rew_flat_map" "in" "*" :=
   autorewrite with rew_flat_map rew_app in *.
 
-Definition ok_Bg (G: Background_LF) : Prop :=
-ok_LF G nil  /\
-ok_LF (flat_map snd_ G) nil.
+Definition ok_Bg_Hyb (G: Background_LF) : Prop :=
+ok_Hyb G nil  /\
+ok_Hyb (flat_map snd_ G) nil.
 
 Fixpoint used_t_vars (G: Background_LF) :=
 match G with
@@ -163,13 +163,13 @@ auto.
 Qed.
 
 
-(* ok_LF for a generic type *)
+(* ok_Hyb for a generic type *)
 
-Lemma ok_LF_used_permut:
+Lemma ok_Hyb_used_permut:
 forall A G U U',
   U *=* U' ->
-  (@ok_LF A G U) ->
-  (@ok_LF A G U').
+  (@ok_Hyb A G U) ->
+  (@ok_Hyb A G U').
 induction G; intros.
 destruct U'; econstructor; eauto.
 destruct a; inversion H0; subst;
@@ -177,34 +177,34 @@ constructor; [ intro | apply IHG with (U:=v::U)]; auto;
 apply Mem_permut with (l':=U) in H1; [ elim H5 | symmetry]; auto.
 Qed.
 
-Lemma ok_LF_used_weakening:
+Lemma ok_Hyb_used_weakening:
 forall A G x U,
-  (@ok_LF A G (x::U)) ->
-  (@ok_LF A G U).
+  (@ok_Hyb A G (x::U)) ->
+  (@ok_Hyb A G U).
 induction G; intros; try constructor;
 destruct a; inversion H; subst;
 constructor.
 intro; apply Mem_permut with (l':=U) in H0; auto; elim H4;
 rewrite Mem_cons_eq; right; auto.
-apply ok_LF_used_permut with (U' := (x::v::U)) in H5;
+apply ok_Hyb_used_permut with (U' := (x::v::U)) in H5;
 [ | permut_simpl]; apply IHG with (x:=x); auto.
 Qed.
 
-Lemma ok_LF_split:
+Lemma ok_Hyb_split:
 forall A G1 G2 U,
-  (@ok_LF A (G1++G2) U) ->
-  ok_LF G1 U /\ ok_LF G2 U.
-induction G1; intros; split; try destruct a; auto using ok_LF.
+  (@ok_Hyb A (G1++G2) U) ->
+  ok_Hyb G1 U /\ ok_Hyb G2 U.
+induction G1; intros; split; try destruct a; auto using ok_Hyb.
 rew_app in *; inversion H; subst; constructor; auto;
 eapply IHG1 with (G2:=G2); auto.
 rew_app in *; inversion H; subst; eapply IHG1 with (G2:=G2); auto;
-eapply ok_LF_used_weakening in H5; eauto.
+eapply ok_Hyb_used_weakening in H5; eauto.
 Qed.
 
 
-(* ok_LF for a specific type -- would be nice to make it more general btw *)
+(* ok_Hyb for a specific type -- would be nice to make it more general btw *)
 
-Add Morphism (@ok_LF (list (var*ty))) : ok_LF_PPermut_lst_var_ty.
+Add Morphism (@ok_Hyb (list (var*ty))) : ok_Hyb_PPermut_lst_var_ty.
 intros x y H; induction H.
 intros; tauto.
 split; intros; inversion H1; subst; constructor; auto;
@@ -215,55 +215,86 @@ intro; elim H8; rewrite Mem_cons_eq; right; auto.
 constructor.
   intro; rewrite Mem_cons_eq in H2; elim H6; destruct H2.
   subst; elim H8; rewrite Mem_cons_eq; left; auto. auto.
-  apply ok_LF_used_permut with (U:=w'::w::y0); auto; permut_simpl.
+  apply ok_Hyb_used_permut with (U:=w'::w::y0); auto; permut_simpl.
 intro; elim H8; rewrite Mem_cons_eq; right; auto.
 constructor.
   intro; rewrite Mem_cons_eq in H2; elim H6; destruct H2.
   subst; elim H8; rewrite Mem_cons_eq; left; auto. auto.
-  apply ok_LF_used_permut with (U:=w::w'::y0); auto; permut_simpl.
+  apply ok_Hyb_used_permut with (U:=w::w'::y0); auto; permut_simpl.
 split; intros.
   apply IHPPermut2; apply IHPPermut1; auto.
   apply IHPPermut1; apply IHPPermut2; auto.
 Qed.
 
-Lemma ok_LF_permut_any:
-forall X (G: list (var * X)) G',
-  G *=* G' ->
-  forall U, ok_LF G U <-> ok_LF G' U.
-(* FIXME: once ~=~ is defined simpler, we can show that *=* -> ~=~ and
-   from that and the above result get the final conclusion;
-   This will be therefore skipped for now *)
-Admitted. (* !!! Bug: #40 *)
-
-Lemma ok_LF_PPermut_ty:
-forall G G'
-  (H: G ~=~ G'),
-  forall U, ok_LF (flat_map snd_ G) U <->
-  ok_LF (flat_map snd_ G') U.
-intros; eapply ok_LF_permut_any; apply flat_map_ppermut; auto.
+Lemma ok_Hyb_permut_any0:
+forall X (G1: list (var * X)) G2 U,
+  G1 *=* G2 ->
+  ok_Hyb G1 U ->
+  ok_Hyb G2 U.
+intro A.
+induction G1; intros.
+apply permut_nil_eq in H; subst; auto.
+destruct a. inversion H0; subst.
+assert ((v, a)::G1 *=* G2) by auto.
+apply permut_split_head in H.
+destruct H as (hd, (tl, H)).
+assert (G1 *=* hd ++ tl).
+  apply permut_cons_inv with (a:=(v, a)); rewrite H1; subst; permut_simpl.
+specialize IHG1 with (G2:=hd++tl).
+apply IHG1 in H6; auto.
+subst; generalize dependent G1; generalize dependent U;
+induction hd; intros; rew_app in *.
+constructor; auto.
+destruct a0. inversion H6; subst. constructor.
+intro; elim H8; rewrite Mem_cons_eq; right; auto.
+apply IHhd with (G1:=hd++tl); try permut_simpl.
+intro n; elim H8; rewrite Mem_cons_eq in n; destruct n; rewrite Mem_cons_eq;
+[left; subst; auto | contradiction].
+apply ok_Hyb_used_permut with (U:=v0::v::U); [permut_simpl | auto].
+intros; auto.
+constructor.
+intro; elim H8; rewrite Mem_cons_eq; rewrite Mem_cons_eq in H; destruct H;
+subst. left; auto. contradiction.
+apply ok_Hyb_used_permut with (U:=v0::v::U); [permut_simpl | auto].
 Qed.
 
-Lemma ok_LF_fresh_te_list:
+Lemma ok_Hyb_permut_any:
+forall X (G: list (var * X)) G',
+  G *=* G' ->
+  forall U, ok_Hyb G U <-> ok_Hyb G' U.
+split; intros; [ | symmetry in H]; eapply ok_Hyb_permut_any0; eauto.
+Qed. (* !!! Bug: #40 *)
+
+Lemma ok_Hyb_PPermut_ty:
+forall G G'
+  (H: G ~=~ G'),
+  forall U, ok_Hyb (flat_map snd_ G) U <->
+  ok_Hyb (flat_map snd_ G') U.
+intros; eapply ok_Hyb_permut_any; apply flat_map_ppermut; auto.
+Qed.
+
+Lemma ok_Hyb_fresh_te_list:
 forall G Gamma v A w U,
- ok_LF ((w, Gamma) :: G) U ->
+ ok_Hyb ((w, Gamma) :: G) U ->
  v \notin (used_t_vars ((w,Gamma)::G)) ->
- ok_LF ((w, (v,A)::Gamma) :: G) U.
+ ok_Hyb ((w, (v,A)::Gamma) :: G) U.
 intros; inversion H; subst; constructor; auto.
 Qed.
 
-Lemma ok_LF_fresh_te_ty:
+Lemma ok_Hyb_fresh_te_ty:
 forall U Gamma G v A w,
- ok_LF (flat_map snd_ ((w, Gamma) :: G)) U ->
+ ok_Hyb (flat_map snd_ ((w, Gamma) :: G)) U ->
  v \notin (used_t_vars ((w, Gamma)::G) \u from_list U) ->
- ok_LF (flat_map snd_ ((w, (v, A)::Gamma) :: G)) U.
+ ok_Hyb (flat_map snd_ ((w, (v, A)::Gamma) :: G)) U.
+intros. remember (flat_map snd_
 (* This proof should be somewhat similar to the one below *)
 Admitted. (*!!! Bug: #41 *)
 
-Lemma ok_LF_fresh_wo_list:
+Lemma ok_Hyb_fresh_wo_list:
 forall G w U l,
- ok_LF G U ->
+ ok_Hyb G U ->
  w \notin (used_w_vars G)  \u from_list U ->
- ok_LF ((w, l) :: G) U.
+ ok_Hyb ((w, l) :: G) U.
 induction G; intros.
 constructor.
   apply notin_Mem; auto.
@@ -276,9 +307,9 @@ destruct a; inversion H; subst; constructor.
   simpl in H0; repeat rewrite notin_union in H0; destruct H0;
   destruct H0; rewrite notin_singleton in H0; elim H0; auto.
   contradiction.
-apply ok_LF_used_permut with (U:=w::v::U).
+apply ok_Hyb_used_permut with (U:=w::v::U).
 permut_simpl.
-assert (ok_LF ((w, l) :: G) (v::U)).
+assert (ok_Hyb ((w, l) :: G) (v::U)).
 apply IHG; auto.
 simpl in *; repeat rewrite notin_union in H0;
 rewrite from_list_cons; repeat rewrite notin_union;
@@ -286,175 +317,175 @@ destruct H0; destruct H0; split; auto; split; auto.
 inversion H1; subst; auto.
 Qed.
 
-Lemma ok_LF_fresh_wo_ty:
+Lemma ok_Hyb_fresh_wo_ty:
 forall G w U,
- ok_LF (flat_map snd_ G) U ->
+ ok_Hyb (flat_map snd_ G) U ->
  w \notin (used_w_vars G) \u from_list U ->
- ok_LF (flat_map snd_ ((w, nil) :: G)) U.
+ ok_Hyb (flat_map snd_ ((w, nil) :: G)) U.
 intros; inversion H; subst; simpl in *; rew_app in *; auto.
 Qed.
 
-Lemma ok_LF_fresh_wo_te_list:
+Lemma ok_Hyb_fresh_wo_te_list:
 forall U G v A w,
- ok_LF G U ->
+ ok_Hyb G U ->
  w \notin (used_w_vars G) \u from_list U ->
  v \notin (used_t_vars G) ->
- ok_LF ((w, (v,A)::nil) :: G) U.
-intros; apply ok_LF_fresh_te_list;
-[ apply ok_LF_fresh_wo_list | ]; auto.
+ ok_Hyb ((w, (v,A)::nil) :: G) U.
+intros; apply ok_Hyb_fresh_te_list;
+[ apply ok_Hyb_fresh_wo_list | ]; auto.
 simpl; rewrite map_nil; rewrite from_list_nil; rewrite union_empty_l; auto.
 Qed.
 
-Lemma ok_LF_fresh_wo_te_ty:
+Lemma ok_Hyb_fresh_wo_te_ty:
 forall U G v A w,
- ok_LF (flat_map snd_ G) U ->
+ ok_Hyb (flat_map snd_ G) U ->
  w \notin (used_w_vars G) \u from_list U ->
  v \notin (used_t_vars G) \u from_list U ->
- ok_LF (flat_map snd_ ((w, (v,A) :: nil) :: G)) U.
-intros; apply ok_LF_fresh_te_ty.
-apply ok_LF_fresh_wo_ty; auto.
+ ok_Hyb (flat_map snd_ ((w, (v,A) :: nil) :: G)) U.
+intros; apply ok_Hyb_fresh_te_ty.
+apply ok_Hyb_fresh_wo_ty; auto.
 simpl; rewrite map_nil; rewrite from_list_nil; rewrite union_empty_l; auto.
 Qed.
 
-Lemma ok_LF_empty_first_list:
+Lemma ok_Hyb_empty_first_list:
 forall w G Gamma U,
-  ok_LF ((w,Gamma) :: G) U ->
-  ok_LF ((w, (@nil (prod var ty))) :: G) U.
+  ok_Hyb ((w,Gamma) :: G) U ->
+  ok_Hyb ((w, (@nil (prod var ty))) :: G) U.
 intros; simpl in *; inversion H; subst; constructor; auto.
 Qed.
 
-Lemma ok_LF_empty_first_ty:
+Lemma ok_Hyb_empty_first_ty:
 forall Gamma (w: var) G U,
-  (@ok_LF ty (flat_map snd_ ((w,Gamma) :: G)) U) ->
-  (@ok_LF ty (flat_map snd_ ((w, nil) :: G)) U).
+  (@ok_Hyb ty (flat_map snd_ ((w,Gamma) :: G)) U) ->
+  (@ok_Hyb ty (flat_map snd_ ((w, nil) :: G)) U).
 induction Gamma; intros; simpl in *; auto; destruct a;
 rew_app in H; inversion H; subst.
 apply IHGamma; auto.
-apply ok_LF_used_weakening with (x:=v); auto.
+apply ok_Hyb_used_weakening with (x:=v); auto.
 Qed.
 
-(* ok_Bg *)
+(* ok_Bg_Hyb *)
 
-Add Morphism ok_Bg : ok_Bg_PPermut.
-intros; unfold ok_Bg; split; intros;
+Add Morphism ok_Bg_Hyb : ok_Bg_Hyb_PPermut.
+intros; unfold ok_Bg_Hyb; split; intros;
 destruct H0; split;
 [ rewrite <- H | |
-  rewrite H | eapply ok_LF_PPermut_ty; try symmetry ]; eauto.
-assert (x ~=~y) by auto; eapply flat_map_ppermut in H; eapply ok_LF_PPermut_ty;
+  rewrite H | eapply ok_Hyb_PPermut_ty; try symmetry ]; eauto.
+assert (x ~=~y) by auto; eapply flat_map_ppermut in H; eapply ok_Hyb_PPermut_ty;
 try symmetry; eauto.
-assert (x ~=~ y) by auto; eapply flat_map_ppermut in H; eapply ok_LF_PPermut_ty;
+assert (x ~=~ y) by auto; eapply flat_map_ppermut in H; eapply ok_Hyb_PPermut_ty;
 eauto.
 Qed.
 
-Lemma ok_Bg_ppermut:
+Lemma ok_Bg_Hyb_ppermut:
 forall G G',
   G ~=~ G' ->
-  ok_Bg G ->
-  ok_Bg G'.
+  ok_Bg_Hyb G ->
+  ok_Bg_Hyb G'.
 intros; rewrite <- H; auto.
 Qed.
 
-Lemma ok_Bg_permut:
+Lemma ok_Bg_Hyb_permut:
 forall G Ctx Ctx' w,
   Ctx *=* Ctx' ->
-  ok_Bg ((w, Ctx) :: G) ->
-  ok_Bg ((w, Ctx') :: G).
+  ok_Bg_Hyb ((w, Ctx) :: G) ->
+  ok_Bg_Hyb ((w, Ctx') :: G).
 intros;
 assert ((w, Ctx) :: G ~=~ (w, Ctx') :: G) by PPermut_simpl;
 rewrite <- H1; auto.
 Qed.
 
-Lemma ok_Bg_permut_last:
+Lemma ok_Bg_Hyb_permut_last:
 forall G Ctx Ctx' w,
   Ctx *=* Ctx' ->
-  ok_Bg (G ++ (w, Ctx) :: nil) ->
-  ok_Bg (G ++ (w, Ctx') :: nil).
+  ok_Bg_Hyb (G ++ (w, Ctx) :: nil) ->
+  ok_Bg_Hyb (G ++ (w, Ctx') :: nil).
 intros;
 assert (G & (w, Ctx) ~=~ G & (w, Ctx')) by PPermut_simpl;
 rewrite <- H1; auto.
 Qed.
 
-Lemma ok_Bg_fresh_te:
+Lemma ok_Bg_Hyb_fresh_te:
 forall G Gamma v A w,
- ok_Bg ((w, Gamma) :: G) ->
+ ok_Bg_Hyb ((w, Gamma) :: G) ->
  v \notin (used_t_vars ((w,Gamma)::G)) ->
- ok_Bg ((w, (v,A)::Gamma) :: G).
-intros; unfold ok_Bg in *;  destruct H; split;
-[ apply ok_LF_fresh_te_list |
-  apply ok_LF_fresh_te_ty]; auto.
+ ok_Bg_Hyb ((w, (v,A)::Gamma) :: G).
+intros; unfold ok_Bg_Hyb in *;  destruct H; split;
+[ apply ok_Hyb_fresh_te_list |
+  apply ok_Hyb_fresh_te_ty]; auto.
 rewrite from_list_nil. rewrite notin_union; split; auto; rewrite notin_empty.
 Qed.
 
-Lemma ok_Bg_fresh_wo:
+Lemma ok_Bg_Hyb_fresh_wo:
 forall G w,
- ok_Bg G ->
+ ok_Bg_Hyb G ->
  w \notin (used_w_vars G) ->
- ok_Bg ((w, nil) :: G).
-intros; unfold ok_Bg in *;  destruct H; split;
-[ eapply ok_LF_fresh_wo_list |
-  eapply ok_LF_fresh_wo_ty]; eauto;
+ ok_Bg_Hyb ((w, nil) :: G).
+intros; unfold ok_Bg_Hyb in *;  destruct H; split;
+[ eapply ok_Hyb_fresh_wo_list |
+  eapply ok_Hyb_fresh_wo_ty]; eauto;
 rewrite from_list_nil; rewrite union_empty_r; auto.
 Qed.
 
-Lemma ok_Bg_fresh_wo_te:
+Lemma ok_Bg_Hyb_fresh_wo_te:
 forall G w v A,
- ok_Bg G ->
+ ok_Bg_Hyb G ->
  w \notin (used_w_vars G) ->
  v \notin (used_t_vars G) ->
- ok_Bg ((w, (v, A) :: nil) :: G).
-intros; unfold ok_Bg in *;  destruct H; split;
-[ apply ok_LF_fresh_wo_te_list |
-  apply ok_LF_fresh_wo_te_ty]; eauto;
+ ok_Bg_Hyb ((w, (v, A) :: nil) :: G).
+intros; unfold ok_Bg_Hyb in *;  destruct H; split;
+[ apply ok_Hyb_fresh_wo_te_list |
+  apply ok_Hyb_fresh_wo_te_ty]; eauto;
 rewrite from_list_nil; rewrite union_empty_r; auto.
 Qed.
 
-Lemma ok_Bg_cons_last:
+Lemma ok_Bg_Hyb_cons_last:
 forall G a,
-  ok_Bg (G & a) <-> ok_Bg (a :: G).
+  ok_Bg_Hyb (G & a) <-> ok_Bg_Hyb (a :: G).
 intros; assert (G & a ~=~ a :: G) by PPermut_simpl;
 rewrite H; split; auto.
 Qed.
 
-Lemma ok_Bg_swap:
+Lemma ok_Bg_Hyb_swap:
 forall C C' G,
-  ok_Bg (C :: G & C') ->
-  ok_Bg (C' :: G & C).
+  ok_Bg_Hyb (C :: G & C') ->
+  ok_Bg_Hyb (C' :: G & C).
 intros; assert (C:: G & C' ~=~ C' :: G & C) by PPermut_simpl;
 rewrite <- H0; auto.
 Qed.
 
-Hint Resolve ok_Bg_cons_last ok_Bg_swap.
-Hint Resolve ok_Bg_permut_last: ok_bg_rew.
-Hint Resolve ok_Bg_fresh_te ok_Bg_fresh_wo ok_Bg_fresh_wo_te.
+Hint Resolve ok_Bg_Hyb_cons_last ok_Bg_Hyb_swap.
+Hint Resolve ok_Bg_Hyb_permut_last: ok_bg_rew.
+Hint Resolve ok_Bg_Hyb_fresh_te ok_Bg_Hyb_fresh_wo ok_Bg_Hyb_fresh_wo_te.
 
-Lemma ok_Bg_permut_first_tail:
+Lemma ok_Bg_Hyb_permut_first_tail:
 forall G C C' w x A,
-  ok_Bg ((w, C) :: G) ->
+  ok_Bg_Hyb ((w, C) :: G) ->
   C *=* (x,A)::C' ->
-  ok_Bg ((w, C') :: G).
+  ok_Bg_Hyb ((w, C') :: G).
 intros;
 assert ((w,(x, A) :: C') :: G ~=~ (w, C) :: G) by PPermut_simpl;
-rewrite <- H1 in H; unfold ok_Bg in *; destruct H; split; simpl in *.
+rewrite <- H1 in H; unfold ok_Bg_Hyb in *; destruct H; split; simpl in *.
 inversion H; subst; constructor; auto.
 rew_app in *; inversion H2; subst; simpl in *.
-apply ok_LF_used_weakening with (x:=x); auto.
+apply ok_Hyb_used_weakening with (x:=x); auto.
 Qed.
-Hint Resolve ok_Bg_permut_first_tail : ok_bg_rew.
+Hint Resolve ok_Bg_Hyb_permut_first_tail : ok_bg_rew.
 
-Lemma ok_Bg_empty_first:
+Lemma ok_Bg_Hyb_empty_first:
 forall w G Gamma,
-  ok_Bg ((w,Gamma) :: G) ->
-  ok_Bg ((w, nil) :: G).
-intros; unfold ok_Bg; destruct H; split;
-[eapply ok_LF_empty_first_list |
- eapply ok_LF_empty_first_ty]; eauto.
+  ok_Bg_Hyb ((w,Gamma) :: G) ->
+  ok_Bg_Hyb ((w, nil) :: G).
+intros; unfold ok_Bg_Hyb; destruct H; split;
+[eapply ok_Hyb_empty_first_list |
+ eapply ok_Hyb_empty_first_ty]; eauto.
 Qed.
 
-Hint Resolve ok_Bg_empty_first : ok_bg_rew.
+Hint Resolve ok_Bg_Hyb_empty_first : ok_bg_rew.
 
-Lemma ok_Bg_Mem_eq:
+Lemma ok_Bg_Hyb_Mem_eq:
 forall w C C' v A A0 G,
-  ok_Bg ((w, C) :: G) ->
+  ok_Bg_Hyb ((w, C) :: G) ->
   C *=* (v, A) :: C' ->
   Mem (v, A0) C ->
   A0 = A.
@@ -464,18 +495,18 @@ assert (exists gh, exists gt, C' = gh & (v, A0) ++ gt) by
     intro HH; inversion HH; subst; elim n; auto);
 destruct H2 as (gh); destruct H2 as (gt); subst;
 assert (C *=* (v, A) :: (v, A0) :: gh ++ gt) by (rewrite H0; permut_simpl);
-unfold ok_Bg in *; destruct H.
-assert (ok_LF (flat_map snd_ ((w, (v, A) :: (v, A0) :: gh ++ gt ) :: G )) nil)
+unfold ok_Bg_Hyb in *; destruct H.
+assert (ok_Hyb (flat_map snd_ ((w, (v, A) :: (v, A0) :: gh ++ gt ) :: G )) nil)
 by
-  (apply ok_LF_PPermut_ty with (G := ((w, C) :: G)); [PPermut_simpl | auto]).
+  (apply ok_Hyb_PPermut_ty with (G := ((w, C) :: G)); [PPermut_simpl | auto]).
 simpl in *. rew_app in *; inversion H4; subst.
 inversion H10; subst;
 elim H11; apply Mem_here.
 Qed.
 
-Lemma ok_Bg_Mem_contradict:
+Lemma ok_Bg_Hyb_Mem_contradict:
 forall A A' w w' v C C' G G',
- ok_Bg ((w, C) :: G) ->
+ ok_Bg_Hyb ((w, C) :: G) ->
  Mem (v, A) C ->
  G ~=~ G' & (w', (v, A') :: C') ->
  False.
@@ -486,68 +517,68 @@ destruct H0 as (gh); destruct H0 as (gt); subst.
 assert ((w, gh & (v, A) ++ gt) :: G' & (w', (v, A') :: C') ~=~
         (w, (v, A) :: gh ++ gt) :: (w', (v, A') :: C') :: G') by
 (PPermut_simpl; apply PPermut_skip; [permut_simpl | auto]).
-rewrite H0 in H; unfold ok_Bg in H; destruct H.
-rew_flat_map in *. simpl ok_LF in H2.
+rewrite H0 in H; unfold ok_Bg_Hyb in H; destruct H.
+rew_flat_map in *. simpl ok_Hyb in H2.
 rew_app in *. inversion H2; subst.
-assert (ok_LF ((v, A') :: C' ++ flat_map snd_ G') (v :: nil)).
-  eapply ok_LF_split with (G1:=flat_map snd_ ((w, gh++gt)::nil)); simpl;
+assert (ok_Hyb ((v, A') :: C' ++ flat_map snd_ G') (v :: nil)).
+  eapply ok_Hyb_split with (G1:=flat_map snd_ ((w, gh++gt)::nil)); simpl;
   rew_app; auto.
 inversion H3; subst; elim H10; apply Mem_here.
 Qed.
 
-Lemma ok_Bg_permut_no_last:
+Lemma ok_Bg_Hyb_permut_no_last:
 forall G w C v A,
-  ok_Bg (G & (w, (v,A) :: C)) ->
-  ok_Bg (G & (w, C)).
+  ok_Bg_Hyb (G & (w, (v,A) :: C)) ->
+  ok_Bg_Hyb (G & (w, C)).
 intros;
 assert (G & (w, C) ~=~ (w,C) :: G) by PPermut_simpl;
 assert (G & (w, (v, A) :: C) ~=~ (w, (v,A) :: C) :: G) by PPermut_simpl;
 rewrite H1 in H; destruct H; simpl in *; split; rew_app in *.
 inversion H; subst; rewrite H0; constructor; auto.
 inversion H2; subst;
-apply ok_LF_PPermut_ty with (U:=nil) in H0;
+apply ok_Hyb_PPermut_ty with (U:=nil) in H0;
 apply H0; simpl;
-apply ok_LF_used_weakening in H8;
+apply ok_Hyb_used_weakening in H8;
 auto.
 Qed.
 
-Lemma ok_Bg_permut_no_last_spec:
+Lemma ok_Bg_Hyb_permut_no_last_spec:
 forall G w C C0 v A,
-  ok_Bg (C0::G & (w, (v,A) :: C)) ->
-  ok_Bg (C0::G & (w, C)).
+  ok_Bg_Hyb (C0::G & (w, (v,A) :: C)) ->
+  ok_Bg_Hyb (C0::G & (w, C)).
 intros;
 assert (C0 :: G & (w, C)  ~=~ (C0 :: G) & (w, C)) by (rew_app; PPermut_simpl);
-rewrite H0; eapply ok_Bg_permut_no_last; rew_app; eauto.
+rewrite H0; eapply ok_Bg_Hyb_permut_no_last; rew_app; eauto.
 Qed.
 
-Lemma ok_Bg_no_last:
+Lemma ok_Bg_Hyb_no_last:
 forall G C,
-  ok_Bg (G & C) -> ok_Bg G.
+  ok_Bg_Hyb (G & C) -> ok_Bg_Hyb G.
 intros;
 assert (G & C ~=~ (C :: nil) ++ G) by PPermut_simpl; rewrite H0 in H;
 destruct H; split.
-eapply ok_LF_split with (G1:=C::nil) (G2:=G); eauto.
+eapply ok_Hyb_split with (G1:=C::nil) (G2:=G); eauto.
 destruct C; rew_app in *; simpl in *.
-eapply ok_LF_split with (G1:=l) (G2:=flat_map snd_  G); auto.
+eapply ok_Hyb_split with (G1:=l) (G2:=flat_map snd_  G); auto.
 Qed.
-Hint Resolve ok_Bg_no_last.
+Hint Resolve ok_Bg_Hyb_no_last.
 
-Lemma ok_Bg_permut_no_last_spec2:
+Lemma ok_Bg_Hyb_permut_no_last_spec2:
 forall G w C C0 v A,
-  ok_Bg (G & (w, (v,A) :: C) & C0) ->
-  ok_Bg (G & (w, C) & C0).
+  ok_Bg_Hyb (G & (w, (v,A) :: C) & C0) ->
+  ok_Bg_Hyb (G & (w, C) & C0).
 intros.
 assert (G & (w, C) & C0 ~=~ G & C0 & (w, C)) by PPermut_simpl;
 rewrite H0;
-apply ok_Bg_permut_no_last with (v:=v) (A:=A).
+apply ok_Bg_Hyb_permut_no_last with (v:=v) (A:=A).
 assert (G & C0 & (w, (v, A) :: C) ~=~ G & (w, (v, A) :: C) & C0)
   by PPermut_simpl;
 rewrite H1; auto.
 Qed.
 
-Lemma ok_Bg_first_last_neq:
+Lemma ok_Bg_Hyb_first_last_neq:
 forall w w' C C' G,
-  ok_Bg ((w, C) :: G & (w', C')) ->
+  ok_Bg_Hyb ((w, C) :: G & (w', C')) ->
   w <> w'.
 intros.
 assert ((w, C) :: G & (w', C') ~=~ (w, C) :: (w', C') :: G) by PPermut_simpl;
@@ -556,9 +587,9 @@ destruct H; simpl in *. inversion H; subst; inversion H7; subst.
 rewrite Mem_cons_eq in H8. rewrite Mem_nil_eq in H8. auto.
 Qed.
 
-Lemma ok_Bg_last_last2_neq:
+Lemma ok_Bg_Hyb_last_last2_neq:
 forall w w' C C' G,
-  ok_Bg (G & (w, C) & (w', C')) ->
+  ok_Bg_Hyb (G & (w, C) & (w', C')) ->
   w <> w'.
 intros;
 assert (G & (w, C) & (w', C') ~=~ (w, C) :: (w', C') :: G) by PPermut_simpl;
@@ -567,10 +598,10 @@ destruct H; simpl in *; inversion H; subst; inversion H7; subst.
 rewrite Mem_cons_eq in H8. rewrite Mem_nil_eq in H8; auto.
 Qed.
 
-Lemma ok_Bg_swap_worlds:
+Lemma ok_Bg_Hyb_swap_worlds:
 forall G w w' C C',
-  ok_Bg (G & (w, C) & (w', C')) ->
-  ok_Bg (G & (w', C) & (w, C')).
+  ok_Bg_Hyb (G & (w, C) & (w', C')) ->
+  ok_Bg_Hyb (G & (w', C) & (w, C')).
 intros.
 assert (G & (w, C) & (w', C') ~=~ (w, C) :: (w', C') :: G) by PPermut_simpl.
 rewrite H0 in H.
@@ -581,52 +612,52 @@ inversion H; subst; constructor. rewrite Mem_nil_eq; tauto.
 inversion H8; subst; constructor.
 rewrite Mem_cons_eq in *; intro; destruct H3; subst;
 [ elim H9; left | rewrite Mem_nil_eq in H3 ]; auto.
-apply ok_LF_used_permut with (U := w'::w::nil); [permut_simpl | ]; auto.
+apply ok_Hyb_used_permut with (U := w'::w::nil); [permut_simpl | ]; auto.
 auto.
 Qed.
 
-Lemma ok_Bg_impl_ppermut:
+Lemma ok_Bg_Hyb_impl_ppermut:
 forall G G' w C C',
-  ok_Bg ((w, C) :: G) ->
+  ok_Bg_Hyb ((w, C) :: G) ->
   G & (w, C) ~=~ G' & (w, C') ->
   G ~=~ G' /\ C *=* C'.
 Admitted. (*!!! Bug: #42 *)
 
 
-(* FIXME: generalize all the ok_Bg_split* into :
-   ok_Bg G <- ok_Bg reorder_G <- ok_Bg reorder_G' <- ok_Bg G':
+(* FIXME: generalize all the ok_Bg_Hyb_split* into :
+   ok_Bg_Hyb G <- ok_Bg_Hyb reorder_G <- ok_Bg_Hyb reorder_G' <- ok_Bg_Hyb G':
    reorder X ~=~ X and all the singletons are in the front *)
 
 
-Lemma ok_Bg_split1:
+Lemma ok_Bg_Hyb_split1:
 forall G w w' C C',
-  ok_Bg ((w,C)::G & (w',C')) ->
-  ok_Bg ((w, C ++ C') :: G).
+  ok_Bg_Hyb ((w,C)::G & (w',C')) ->
+  ok_Bg_Hyb ((w, C ++ C') :: G).
 intros.
 assert ((w, C) :: G & (w', C') ~=~ (w,C) :: (w', C')::G) by PPermut_simpl.
 rewrite H0 in H; destruct H; split; simpl in *.
 inversion H; subst; inversion H7; subst; constructor; auto;
-apply ok_LF_used_weakening with (x:=w'); auto.
+apply ok_Hyb_used_weakening with (x:=w'); auto.
 rew_app; auto.
 Qed.
 
-Lemma ok_Bg_split2:
+Lemma ok_Bg_Hyb_split2:
 forall G w w' C C',
-  ok_Bg ((w,C)::G & (w',C')) ->
-  ok_Bg ((w', C' ++ C) :: G).
+  ok_Bg_Hyb ((w,C)::G & (w',C')) ->
+  ok_Bg_Hyb ((w', C' ++ C) :: G).
 intros.
 assert ((w, C) :: G & (w', C') ~=~ (w', C') :: (w, C)::G) by PPermut_simpl.
 rewrite H0 in H; destruct H; split; simpl in *.
 inversion H; subst; inversion H7; subst;
 constructor; auto.
-apply ok_LF_used_weakening with (x:=w); auto.
+apply ok_Hyb_used_weakening with (x:=w); auto.
 rew_app; auto.
 Qed.
 
-Lemma ok_Bg_split3:
+Lemma ok_Bg_Hyb_split3:
 forall G w w' w'' C C' C'',
-  ok_Bg ((w,C)::G & (w',C') & (w'',C'')) ->
-  ok_Bg ((w, C) :: G & (w', C' ++ C'')).
+  ok_Bg_Hyb ((w,C)::G & (w',C') & (w'',C'')) ->
+  ok_Bg_Hyb ((w, C) :: G & (w', C' ++ C'')).
 intros.
 assert ((w, C) :: G & (w', C') & (w'',C'') ~=~
   (w, C) :: (w', C'):: (w'',C'') :: G) by PPermut_simpl.
@@ -635,14 +666,14 @@ assert ((w,C) :: G & (w', C'++C'') ~=~ (w,C) :: (w', C'++C'') :: G)
 rewrite H0 in H; rewrite H1; destruct H; split; simpl in *.
 inversion H; subst; inversion H8; subst; inversion H10; subst;
 constructor; auto; constructor; auto.
-apply ok_LF_used_weakening with (x:=w''); auto.
+apply ok_Hyb_used_weakening with (x:=w''); auto.
 rew_app; auto.
 Qed.
 
-Lemma ok_Bg_split4:
+Lemma ok_Bg_Hyb_split4:
 forall G w w' C C',
-  ok_Bg (G & (w, C) & (w', C')) ->
-  ok_Bg (G & (w', C' ++ C)).
+  ok_Bg_Hyb (G & (w, C) & (w', C')) ->
+  ok_Bg_Hyb (G & (w', C' ++ C)).
 intros.
 assert (G & (w, C) & (w', C') ~=~
   (w, C) :: (w', C') :: G) by PPermut_simpl.
@@ -651,19 +682,19 @@ assert (G & (w', C'++C) ~=~ (w', C'++C) :: G)
 rewrite H0 in H; rewrite H1; destruct H; split.
 simpl in *; inversion H; subst; inversion H8; subst; constructor; auto.
 rewrite Mem_nil_eq; tauto.
-apply ok_LF_used_weakening with (x:=w);
-apply ok_LF_used_permut with (U:= w'::w::nil);
+apply ok_Hyb_used_weakening with (x:=w);
+apply ok_Hyb_used_permut with (U:= w'::w::nil);
 try permut_simpl; auto.
 assert ((w', C'++C)::G ~=~ (w',C++C')::G) by PPermut_simpl.
-apply ok_LF_PPermut_ty with (U:=nil) in H3.
+apply ok_Hyb_PPermut_ty with (U:=nil) in H3.
 simpl in *; rew_app in *.
 apply H3. auto.
 Qed.
 
-Lemma ok_Bg_split5:
+Lemma ok_Bg_Hyb_split5:
 forall G w w' C C',
-  ok_Bg (G & (w, C) & (w', C')) ->
-  ok_Bg (G & (w, C ++ C')).
+  ok_Bg_Hyb (G & (w, C) & (w', C')) ->
+  ok_Bg_Hyb (G & (w, C ++ C')).
 intros.
 assert (G & (w, C) & (w', C') ~=~
   (w, C) :: (w', C') :: G) by PPermut_simpl.
@@ -672,14 +703,14 @@ assert (G & (w, C++C') ~=~ (w, C++C') :: G)
 rewrite H0 in H; rewrite H1; destruct H; split; simpl in *.
 inversion H; subst; inversion H8; subst.
 constructor; auto;
-apply ok_LF_used_weakening with (x:=w'); auto.
+apply ok_Hyb_used_weakening with (x:=w'); auto.
 rew_app; auto.
 Qed.
 
-Lemma ok_Bg_split6:
+Lemma ok_Bg_Hyb_split6:
 forall G w C C' C'' w' w'',
-  ok_Bg (G & (w, C) & (w', C') & (w'', C'')) ->
-  ok_Bg (G & (w, C ++ C') & (w'', C'')).
+  ok_Bg_Hyb (G & (w, C) & (w', C') & (w'', C'')) ->
+  ok_Bg_Hyb (G & (w, C ++ C') & (w'', C'')).
 intros.
 assert (G & (w,C) & (w', C') & (w'',C'') ~=~
   (w, C) :: (w', C'):: (w'',C'') :: G) by PPermut_simpl.
@@ -688,21 +719,21 @@ assert (G & (w, C++C') & (w'', C'') ~=~ (w, C ++ C') :: (w'', C'') :: G)
 rewrite H0 in H; rewrite H1; destruct H; split; simpl in *.
 inversion H; subst; inversion H8; subst; inversion H10; subst.
 constructor; auto.
-apply ok_LF_used_weakening with (x:=w'); auto.
+apply ok_Hyb_used_weakening with (x:=w'); auto.
 rew_app; auto.
 Qed.
 
 (* This is actually false
-Lemma ok_Bg_split7:
+Lemma ok_Bg_Hyb_split7:
 forall G w w' w'' C C' C'',
-  ok_Bg ((w,C)::G & (w'',C'')) ->
-  ok_Bg ((w, C ++ C'') :: G & (w', C')).
+  ok_Bg_Hyb ((w,C)::G & (w'',C'')) ->
+  ok_Bg_Hyb ((w, C ++ C'') :: G & (w', C')).
 *)
 
-Lemma ok_Bg_split8:
+Lemma ok_Bg_Hyb_split8:
 forall G G' w w' w'' C C' C'',
-  ok_Bg (G ++ G' ++ (w, C) :: (w', C') :: (w'', C'') :: nil) ->
-  ok_Bg (G ++ G' ++ (w', C') :: (w'', C'' ++ C)::nil) .
+  ok_Bg_Hyb (G ++ G' ++ (w, C) :: (w', C') :: (w'', C'') :: nil) ->
+  ok_Bg_Hyb (G ++ G' ++ (w', C') :: (w'', C'' ++ C)::nil) .
 intros.
 assert (G++G' ++ (w, C) :: (w', C') :: (w'',C'') :: nil ~=~
   (w, C) :: (w', C'):: (w'',C'') :: G ++ G') by PPermut_simpl.
@@ -719,19 +750,19 @@ intro; elim H11; rewrite Mem_cons_eq in *; destruct H3.
 left; auto.
 rewrite Mem_nil_eq in H3; auto.
 contradiction.
-apply ok_LF_used_weakening with (x:=w);
-apply ok_LF_used_permut with (U:=w'' :: w' :: w :: nil);
+apply ok_Hyb_used_weakening with (x:=w);
+apply ok_Hyb_used_permut with (U:=w'' :: w' :: w :: nil);
 auto; permut_simpl.
-apply ok_LF_PPermut_ty with (G':=(w',C') :: (w'', C'')::(w,C) :: G ++ G') in H2.
+apply ok_Hyb_PPermut_ty with (G':=(w',C') :: (w'', C'')::(w,C) :: G ++ G') in H2.
 simpl in *.
 rew_app. auto.
 PPermut_simpl.
 Qed.
 
-Lemma ok_Bg_split9:
+Lemma ok_Bg_Hyb_split9:
 forall G w w' w'' C C' C'',
-  ok_Bg ((w,C)::G & (w',C') & (w'',C'')) ->
-  ok_Bg ((w, C++C') :: G & (w'', C'')).
+  ok_Bg_Hyb ((w,C)::G & (w',C') & (w'',C'')) ->
+  ok_Bg_Hyb ((w, C++C') :: G & (w'', C'')).
 intros.
 assert ((w, C) :: G & (w', C') & (w'',C'') ~=~
   (w, C) :: (w', C'):: (w'',C'') :: G) by PPermut_simpl.
@@ -744,16 +775,16 @@ constructor; auto; constructor.
 intro; rewrite Mem_cons_eq in *. destruct H3; subst.
 elim H11;right; apply Mem_here.
 rewrite Mem_nil_eq in H3; auto.
-apply ok_LF_used_weakening with (x:=w');
-apply ok_LF_used_permut with (U:=w'' :: w' :: w :: nil);
+apply ok_Hyb_used_weakening with (x:=w');
+apply ok_Hyb_used_permut with (U:=w'' :: w' :: w :: nil);
 auto; permut_simpl.
 rew_app. auto.
 Qed.
 
-Lemma ok_Bg_split10:
+Lemma ok_Bg_Hyb_split10:
 forall G G' w1 w2 w3 w4 c1 c2 c3 c4,
-  ok_Bg (G ++ (w1, c1)::G' ++ (w2, c2) :: (w3, c3) :: (w4, c4) :: nil) ->
-  ok_Bg (G ++ (w1, c1)::G' ++ (w2, c2 ++ c3) :: (w4, c4) :: nil).
+  ok_Bg_Hyb (G ++ (w1, c1)::G' ++ (w2, c2) :: (w3, c3) :: (w4, c4) :: nil) ->
+  ok_Bg_Hyb (G ++ (w1, c1)::G' ++ (w2, c2 ++ c3) :: (w4, c4) :: nil).
 intros.
 assert (G ++ (w1,c1) :: G' ++ (w2, c2) :: (w3, c3) :: (w4,c4) :: nil ~=~
    (w1,c1) :: (w2, c2) :: (w3, c3) :: (w4,c4) :: G ++ G') by PPermut_simpl.
@@ -768,18 +799,18 @@ elim H13; right; left; auto.
 rewrite Mem_cons_eq in H3; destruct H3; subst.
 elim H13; right; rewrite Mem_cons_eq; right; rewrite Mem_cons_eq; left; auto.
 rewrite Mem_nil_eq in H3; auto.
-apply ok_LF_used_weakening with (x:=w3);
-apply ok_LF_used_permut with (U:=w4 :: w3 :: w2 :: w1 :: nil);
+apply ok_Hyb_used_weakening with (x:=w3);
+apply ok_Hyb_used_permut with (U:=w4 :: w3 :: w2 :: w1 :: nil);
 auto; permut_simpl.
 rew_app; auto.
 Qed.
 
-Hint Resolve ok_Bg_split1 ok_Bg_split2 ok_Bg_split3 ok_Bg_split4
-  ok_Bg_split5 ok_Bg_split6 ok_Bg_split8
-  ok_Bg_split9 ok_Bg_split10 : ok_bg_rew.
-Hint Resolve ok_Bg_permut_no_last ok_Bg_permut_no_last_spec2
-  ok_Bg_permut_no_last_spec ok_Bg_first_last_neq
-  ok_Bg_last_last2_neq : ok_bg_rew.
-Hint Resolve ok_Bg_swap_worlds.
+Hint Resolve ok_Bg_Hyb_split1 ok_Bg_Hyb_split2 ok_Bg_Hyb_split3 ok_Bg_Hyb_split4
+  ok_Bg_Hyb_split5 ok_Bg_Hyb_split6 ok_Bg_Hyb_split8
+  ok_Bg_Hyb_split9 ok_Bg_Hyb_split10 : ok_bg_rew.
+Hint Resolve ok_Bg_Hyb_permut_no_last ok_Bg_Hyb_permut_no_last_spec2
+  ok_Bg_Hyb_permut_no_last_spec ok_Bg_Hyb_first_last_neq
+  ok_Bg_Hyb_last_last2_neq : ok_bg_rew.
+Hint Resolve ok_Bg_Hyb_swap_worlds.
 
 Close Scope permut_scope.
